...뭔가 잘못했어. 다시 해야지.

src/02-Introduction-to-Semantics/Lecture02.ReflexiveTransitiveClosure.fst
@@ -1,16 +1,124 @@
 module Lecture02.ReflexiveTransitiveClosure
 
-(*
+open Lecture02.BinaryRelation { (∈) } 
 module Br = Lecture02.BinaryRelation
 module Rule = Lecture02.InferenceRule
+module RuleBuilder = Lecture02.InferenceRule.Builder
 module L = FStar.List.Tot
+
+
+type step_t (state_t:eqtype) = (state_t & state_t)
+type small_step_relation_t (state_t:eqtype) = Br.binary_relation_t (Br.to_set state_t) (Br.to_set state_t)
+
+noeq
+type raw_builder_t 
+  #state_t (model_t:Type) (small_step_relation:small_step_relation_t state_t) =
+| ConclusionOnly: 
+    (to_conclusion:model_t -> (step_t state_t)) -> 
+    (raw_builder_t model_t small_step_relation)
+| AddPremise: 
+    (to_premise:model_t -> (step_t state_t)) ->
+    (raw_builder_t model_t small_step_relation) ->
+    (raw_builder_t model_t small_step_relation)
+
+
+let rec get_conclusion_from_raw
+  #state_t (#model_t:Type) (#small_step_relation:small_step_relation_t state_t)
+  (raw_builder:raw_builder_t model_t small_step_relation)
+  (model:model_t)
+  : Tot (step_t state_t) (decreases raw_builder) =
+  match raw_builder with
+  | ConclusionOnly tc -> tc model
+  | AddPremise tp pre_raw_builder -> get_conclusion_from_raw pre_raw_builder model
+
+let is_example
+  #state_t (#model_t:Type) (#small_step_relation:small_step_relation_t state_t)
+  (raw_builder:raw_builder_t model_t small_step_relation)
+  (model:model_t)
+  : prop =
+  match raw_builder with
+  | ConclusionOnly tc -> let s = tc model in (fst s) = (snd s)
+  | AddPremise tp pre_raw_builder ->
+  let s1 = tp model in
+  let s2 = get_conclusion_from_raw pre_raw_builder model in
+  let s3 = get_conclusion_from_raw raw_builder model in
+  (s1 ∈ small_step_relation) /\
+  ((fst s1) = (fst s3)) /\ ((snd s1) = (fst s2)) /\ ((snd s2) = (snd s3))
+
+let is_valid
+  #state_t (#model_t:Type) (#small_step_relation:small_step_relation_t state_t)
+  (raw_builder:raw_builder_t model_t small_step_relation)
+  : prop =
+  forall (model:model_t). (is_example raw_builder model)
+
+type builder_t 
+  #state_t (model_t:Type) (small_step_relation:small_step_relation_t state_t) =
+  x:(raw_builder_t model_t small_step_relation){is_valid x}
+
+private let rec to_rule_builder_core
+  #state_t (#model_t:Type) (#small_step_relation:small_step_relation_t state_t)
+  (raw_builder:raw_builder_t model_t small_step_relation) (lub_builder:builder_t model_t small_step_relation)
+  : Pure (RuleBuilder.t model_t) 
+    (requires (raw_builder == lub_builder) \/ (raw_builder << lub_builder))
+    (ensures fun r -> True)
+    (decreases raw_builder) =
+  match raw_builder with
+  | ConclusionOnly to_conclusion -> RuleBuilder.ConclusionOnly {
+      meta_proposition_t = step_t state_t;
+      apply = to_conclusion;
+      hold = fun x -> 
+        forall (model:model_t). (get_conclusion_from_raw lub_builder model) = (to_conclusion model)
+    }
+  | AddPremise to_premise pre_raw_builder ->
+    let new_premise : RuleBuilder.meta_proposition_schema_t model_t = {
+      meta_proposition_t = step_t state_t;
+      apply = to_premise;
+      hold = fun x -> (x ∈ small_step_relation)
+    } 
+    in
+    let pre_rule_builder = to_rule_builder_core pre_raw_builder lub_builder in
+    RuleBuilder.AddPremise new_premise pre_rule_builder
+
+let to_rule_builder
+  #state_t (#model_t:Type) (#small_step_relation:small_step_relation_t state_t)
+  (builder:builder_t model_t small_step_relation)
+  : Tot (RuleBuilder.t model_t) =
+  to_rule_builder_core builder builder
+
+let build
+  #state_t (#model_t:Type) (#small_step_relation:small_step_relation_t state_t)
+  (builder:builder_t model_t small_step_relation)
+  : Rule.t model_t =
+  RuleBuilder.build (to_rule_builder builder)
+
+open FStar.Tactics.V2
+let lemma_build 
+  #state_t (#model_t:Type) (#small_step_relation:small_step_relation_t state_t)
+  (builder:builder_t model_t small_step_relation)
+  : Lemma (Rule.is_valid (build builder)) =
+  //assert (Rule.is_valid (build builder)) by (dump "")
+  admit ()
+  (* 역시, 이게 그냥은 증명이 안 되네... *)
 
 type label_t =
 | Refl
 | Trans
 
-type small_step_predicate_t (state_t:eqtype) = Br.binary_predicate_t state_t state_t
+let get_label 
+  #state_t (#model_t:Type) (#small_step_relation:small_step_relation_t state_t)
+  (builder:builder_t model_t small_step_relation)
+  : label_t =
+  match builder with
+  | ConclusionOnly _ -> Refl
+  | AddPremise _ _ -> Trans
 
+
+(* goal: is_multi_step *)
+
+
+
+
+(*
 let is_rule 
   (state_t:eqtype)
   (x:Rule.t)
